lean-tracing-demo-ccfraft/Sparse/NativeEncode.lean
@@ -51,10 +51,12 @@ structure Columns where
   hasJoined : Nat := 16
   preVoteStatus : Nat := 17
   retirementCompleted : Nat := 18
+  submittedTxIds : Nat := 19
+  submittedTxLimit : Nat := 20
 
 structure Encoding (width : PNat) extends Columns where
   bootstrap : BitVec width
-  next : Nat := 19
+  next : Nat := 21
   assertions : Array (Expr .bool) := #[]
   symbolsBounded : forall formula, formula ∈ assertions ->
     forall symbol, symbol ∈ formula.symbols -> symbol.2 < next
